concurrency/compiler/synchronisation_symulations.v
@@ -6351,4 +6351,3 @@ Qed.
   End SyncCallsDiagrams.
   
 End SyncSimulation.
-
